Ownership-NoIncoming.dfy
@@ -40,34 +40,34 @@ lemma {:isolate_assertions} ShorterNoIncomingPointers(f : Object, o : Object, t 
 
    ensures not(refOK(f,t))
 {
-  //assert f != t;
-//
-//  assert outside(f,t);  assert not(inside(f,t));
-//
-// //    assert refOK(f,t)  ==> ((f==t) || refBI(f,t) || refDI(f,t));
-// //    assert refOK(f,t) <==  ((f==t) || refBI(f,t) || refDI(f,t));
-//    assert refOK(f,t) <==> ((f==t) || refBI(f,t) || refDI(f,t));
-//
-//    assert not(f==t);
-//    assert not(refBI(f,t));
+  assert f != t;
 
-//    if (refDI(f,t)) {
-// //      assert f in t.owner;
-// //      DreddOwner(f,t);
-//     //   assert inside(t,f);
-//     //   assert outside(t,f);
-//
-//     //   assert t == f;
-//     //   assert t != f;
-//
-// //      assert false;
-//    } else {
-//
-// //    assert not(refDI(f,t));
-// //   assert not(refOK(f,t));
-//    }
+ assert outside(f,t);  assert not(inside(f,t));
 
-// assert not(refOK(f,t));
+   assert refOK(f,t)  ==> ((f==t) || refBI(f,t) || refDI(f,t));
+   assert refOK(f,t) <==  ((f==t) || refBI(f,t) || refDI(f,t));
+   assert refOK(f,t) <==> ((f==t) || refBI(f,t) || refDI(f,t));
+
+   assert not(f==t);
+   assert not(refBI(f,t));
+
+   if (refDI(f,t)) {
+     assert f in t.owner;
+     DreddOwner(f,t);
+      assert inside(t,f);
+  //    assert outside(t,f);
+
+//       assert t == f;
+//       assert t != f;
+//
+//      assert false;
+   } else {
+
+   assert not(refDI(f,t));
+  assert not(refOK(f,t));
+   }
+
+assert not(refOK(f,t));
 }
 
 
@@ -115,4 +115,22 @@ lemma {:isolate_assertions} LongerNoIncomingPointers(f : Object, o : Object, t :
    }
 
  assert not(refOK(f,t));
+}
+
+
+
+lemma {:isolate_assertions } fint_refDI_outside(f : Object, t : Object)
+  requires f.Ready()
+  requires t.Ready()
+  requires t.owner == {f}
+   ensures refDI_fall(f,t)
+   ensures refDI_seqo(f,t)
+    // ensures refDI_fint(f,t)
+  ensures refDI(f,t)
+  ensures refOK(f,t)
+  ensures flatten(f.self) == flatten(t.owner)
+{
+     DreddOwner(f,t);
+      assert inside(t,f);
+//    assert outside(t,f);
 }
